@prefix andr: <http://purl.org/net/andruian/datadef#> .
@prefix sp: <http://spinrdf.org/sp#> .
@prefix s: <http://schema.org/> .
@prefix rdfs: <http://www.w3.org/2000/01/rdf-schema#> .
@prefix rdf: <http://www.w3.org/1999/02/22-rdf-syntax-ns#> .
@prefix xsd: <http://www.w3.org/2001/XMLSchema#> .

###########
# Classes #
###########

andr:DataDef a rdfs:Class;
    rdfs:label "DataDef";
    rdfs:comment """The definition of a single data mapping in the Andruian framework. That is a mapping of Source class 
instances to instances of the Location class. See https://github.com/andruian/example-data for more information.""";
    .
    
andr:LocationClassDef a rdfs:Class;
    rdfs:label "LocationClassDef";
    rdfs:comment """The definition of a Location class and its metadata. That includes the SPARQL endpoint where instances  
of this class may be found and property paths specifying how to get the Location class' latitude and longitude.""";
    .
    
andr:SourceClassDef a rdfs:Class;
    rdfs:label "SourceClassDef";
    rdfs:comment """The definition of a Source class and its metadata. That includes the SPARQL endpoint where instances 
of this class may be found, the property path leading to the linked Location class and properties that should be indexed 
on the index server for faster retrieval.""";
    .
    
andr:SelectPropertyDef a rdfs:Class;
    rdfs:label "SelectPropertyDef";
    rdfs:comment """Definition of a Source class' property that should be indexed on the index server. The definition 
specifies name to use for the property and a property path leading to it.""";
    .
    
andr:IndexServer a rdfs:Class;
    rdfs:label "IndexServer";
    rdfs:comment """An index server for the Andruian framework. It is optional - if not present, clients fall back to 
naive queries. They are slower though.""";
    .

andr:LocationClassPathsSource a rdfs:Class;
    rdfs:label "LocationClassPathsSource";
    rdfs:comment "A source of property paths leading from an instance of a class to its latitude and longitude.";
    .
    
andr:ClassToLocPath a rdfs:Class;
    rdfs:label "ClassToLocPath";
    rdfs:comment "A property path for a particular class leading to its latitude and longitude.";
    .

andr:PropertyPath a rdfs:Class;
    rdfs:label "A path of one or more properties";
    rdfs:comment """This class is equivalent to a predicate sequence SHACL property path.
SHACL does not define a RDFS class for property paths, but only refers to them as to
a plain rdf:Resource. andr:PropertyPath class is defined in Andruian data definition schema
to make the diagram and property domains easily readable.

A predicate or sequence path may be used wherever andr:PropertyPath is expected. A predicate
path is a single property in place of the object; a sequence path is a RDF list containing
two or more properties in place of the object.""".

##############
# Properties #
##############

#
# DataDef 
#
andr:sourceClassDef a rdf:Property;
    rdfs:label   "sourceClassDef";
    rdfs:comment "A definition of the Source Class in the Andruian framework. This class is typically user-defined and links to a Location class.";
    rdfs:range   andr:SourceClassDef;
    rdfs:domain  andr:DataDef;
    .
 
andr:indexServer a rdf:Property;
    rdfs:label "indexServer";
    rdfs:comment "A definition of an Index Server in the Andruian framework. This is an optional property.";
    rdfs:range andr:IndexServer;
    rdfs:domain  andr:DataDef;
    .
    
andr:uri a rdf:Property;
    rdfs:label "uri";
    rdfs:comment "A link where the subject of the property can be accessed.";
    rdfs:range rdf:Resource;
    .
    
andr:version a rdf:Property;
    rdfs:label "version";
    rdfs:comment "An integer representing version of the subject of the property.";
    rdfs:range xsd:integer;
    .

andr:class a rdf:Property;
    rdfs:label "class";
    rdfs:comment "A specification of a resource type (class) relevant to the subject of this property.";
    rdfs:range rdfs:Class;
    .
    
# 
# SourceClassDef 
#    
andr:selectProperty a rdf:Property;
    rdfs:label "selectProperty";
    rdfs:comment "Defines zero or more andr:SelectProperty instances for the subject of this property. This is an optional property, it may be specified multiple times.";
    rdfs:range andr:SelectProperty;
    rdfs:domain  andr:SourceClassDef;
    .
    
andr:propertyPath a rdf:Property;
    rdfs:label "propertyPath";
    rdfs:comment """Defines a property path. The object of this property must be a SHACL predicate or sequence path. See
https://www.w3.org/TR/shacl/#property-path-predicate for more details.""";
    .
    
andr:pathToLocationClass a rdf:Property;
    rdfs:label "pathToLocationClass";
    rdfs:comment """Defines a property path that, when applied to the subject of the property, leads to an instance of 
the Location Class linked to the subject. The object of this property must be a SHACL predicate or sequence path. See
https://www.w3.org/TR/shacl/#property-path-predicate for more details.""";
    rdfs:domain  andr:SourceClassDef;
    .
    
andr:sparqlEndpoint a rdf:Property;
    rdfs:label "sparqlEndpoint";
    rdfs:comment "A definition of an URI where a SPARQL endpoint relevant to the property subject may be reached.";
    rdfs:range rdf:Resource;
    .
    
andr:sourceClassDef a rdf:Property;
    rdfs:label "sourceClassDef";
    rdfs:comment "A Source Class definition for this DataDef.";
    rdfs:range andr:SourceClassDef;
    rdfs:domain  andr:DataDef;
    .
    

#
# LocationClassDef
#
andr:locationClassDef a rdf:Property;
    rdfs:label "locationClassDef";
    rdfs:comment "A Location Class definition for this DataDef.";
    rdfs:range andr:LocationClassDef;
    rdfs:domain  andr:DataDef;
    .
    
andr:locationClassPathsSource a rdf:Property;
    rdfs:label "locationClassPathsSource";
    rdfs:comment """Defines a source object for property paths describing the path from an entity of a given class to the latitude/longitude 
coordinates associated with such class. The object of this property will link to one or more property path definitions.""";
    rdfs:range andr:LocationClassPathsSource;
    rdfs:domain  andr:LocationClassDef;
    .

andr:includeRdf a rdf:Property;
    rdfs:label "includeRdf";
    rdfs:comment """Specifies an URL where an RDF file is located. The consumer of this dataset shall download the linked
file and include the data contained there in their internal model before processing any other properties of the subject.

This property is an analogy to import statements in programming languages - only it imports a remote file.""";
    rdfs:range rdf:Resource;
    rdfs:domain andr:LocationClassDef;
    .
    
andr:classToLocPath a rdf:Property;
    rdfs:label "classToLocPath";
    rdfs:comment "Defines property paths for a single resource type (class), leading from an object of such class to its latitude/longitude.";
    rdfs:range andr:ClassToLocPath;
    .
    
andr:latPath a rdf:Property;
    rdfs:label "latPath";
    rdfs:comment "Defines a property path linking to the latitude coordinate. The object of this property must be a SHACL predicate or sequence path. See https://www.w3.org/TR/shacl/#property-path-predicate for more details.";
    .
    
andr:longPath a rdf:Property;
    rdfs:label "longPath";
    rdfs:comment "Defines a property path linking to the longitude coordinate. The object of this property must be a SHACL predicate or sequence path. See https://www.w3.org/TR/shacl/#property-path-predicate for more details.";
    .